begins

src/MC_CTL.v
@@ -1,30 +1,3 @@
-
-(* 
-
-Inductive ex (A:Type) (P: A -> Prop) : Prop :=
-  ex_intro : forall x:A, forall _: P x, ex A P.
-Inductive ex2 (A:Type) (P Q:A -> Prop) : Prop :=
-  ex_intro2 : forall x:A, P x -> Q x -> ex2 A P Q.
-
-Notation "'exists' x .. y , p" := (ex (fun x => .. (ex (fun y => p)) ..))
-(at level 200, x binder, right associativity,
-  format "'[' 'exists' '/ ' x .. y , '/ ' p ']'")
-: type_scope.
-
-Notation "'exists2' x , p & q" := (ex2 (fun x => p) (fun x => q))
-  (at level 200, x name, p at level 200, right associativity) : type_scope.
-Inductive and (A B : Prop) : Prop :=
-| conj : A -> B -> and A B.
-Notation "A /\ B" := (and A B).
-Inductive or (A B : Prop) : Prop :=
-| or_introl : A -> or A B 
-| or_intror : B -> or A B.
-Notation "A \/ B" := (or A B).
-
-*)
-Check eq _ _ -> eq _ _ .
-Print ex_intro.
-
 Definition cAX: forall X : Type, 
 (X -> X -> Prop) -> (X -> Prop) -> X -> Prop := 
   fun (X : Type) (e : X -> X -> Prop) (p : X -> Prop) (w : X) =>
@@ -70,65 +43,14 @@ Record sts := STS {
   label  : nat -> state -> Prop;
   serial : forall w:state, exists v, trans w v
 }.
-(* Inductive nat : Set :=  S : nat -> nat. *)
-Check ex.
 
 
 Fixpoint satisfies (M : sts) (s : form){struct s}:state M -> Prop := 
   (match s with
   | fF        => fun w : state M => False
-  | fV v      => label M v
+  | fV v      => fun w : state M => label M v w
   | fImp s0 t => fun w : state M => satisfies M s0 w -> satisfies M t w
-  | fAX  s0   => cAX (state M) (trans M) (satisfies M s0)
-  | fAR  s0 t => pAR (state M) (trans M) (satisfies M s0) (satisfies M t)
-  | fAU  s0 t => pAU (state M) (trans M) (satisfies M s0) (satisfies M t)
+  | fAX  s0   => fun w : state M => cAX (state M) (trans M) (satisfies M s0) w
+  | fAR  s0 t => fun w : state M => pAR (state M) (trans M) (satisfies M s0) (satisfies M t) w
+  | fAU  s0 t => fun w : state M => pAU (state M) (trans M) (satisfies M s0) (satisfies M t) w
   end: state M -> Prop ).
-
-Print False.
-
-
-Inductive bool : Set :=  true : bool | false : bool.
-
-Definition trans_bool (s1:bool)(s2:bool):Prop := ~ (s1 = s2).
-Definition label_bool(v: nat)(s:bool):Prop := v = (match s with | false => 0 | true => 1 end).
-Definition serial_bool: forall w:bool, exists v, trans_bool w v.
-intros. case w; [> eexists false|eexists true] ;compute;discriminate.
-Defined.  
-
-Definition init_bool(s: bool):Prop := s = false.
-Definition model_bool: sts :=  {| state := bool; trans := trans_bool; init:= init_bool; label := label_bool; serial := serial_bool |}.
-
-Theorem check1: forall st: state model_bool, 
-(init model_bool) st -> 
-satisfies(model_bool) (fAX (( (fV 1)))) st.
-Proof.
-  compute.
-  intros. destruct v. auto. apply H0 in H. refine (match H with end).
-Defined.
-
-  
-  
-  
-  
-  
-  
-Qed.
-  
-  
-  
-  
-  
-
-  
-  
-  
-  
-  
-  
-
-  
-
-  
-
-Qed.
-	 
