src/listing.v
@@ -1,0 +1,137 @@
+
+(* 
+
+Inductive ex (A:Type) (P: A -> Prop) : Prop :=
+  ex_intro : forall x:A, forall _: P x, ex A P.
+Inductive ex2 (A:Type) (P Q:A -> Prop) : Prop :=
+  ex_intro2 : forall x:A, P x -> Q x -> ex2 A P Q.
+
+Notation "'exists' x .. y , p" := (ex (fun x => .. (ex (fun y => p)) ..))
+(at level 200, x binder, right associativity,
+  format "'[' 'exists' '/ ' x .. y , '/ ' p ']'")
+: type_scope.
+
+Notation "'exists2' x , p & q" := (ex2 (fun x => p) (fun x => q))
+  (at level 200, x name, p at level 200, right associativity) : type_scope.
+Inductive and (A B : Prop) : Prop :=
+| conj : A -> B -> and A B.
+Notation "A /\ B" := (and A B).
+Inductive or (A B : Prop) : Prop :=
+| or_introl : A -> or A B 
+| or_intror : B -> or A B.
+Notation "A \/ B" := (or A B).
+
+Inductive le (n : nat) : nat -> Prop :=
+	le_n : n <= n | le_S : forall m : nat, n <= m -> n <= S m.
+
+*)
+Locate "_ = _".
+Check @eq_refl nat 1.
+Check eq 0 1.
+(* Inductive eq (A : Type) (x : A) : A -> Prop :=  eq_refl : x = x. *)
+Inductive ex (A:Type) (P: A -> Prop) : Prop :=
+  ex_intro : forall x:A, forall _: P x, ex A P.
+Inductive ex2 (A:Type) (P Q:A -> Prop) : Prop :=
+  ex_intro2 : forall x:A, P x -> Q x -> ex2 A P Q.
+(* Inductive le (n : nat) : nat -> Prop :=
+	le_n : n <= n | le_S : forall m : nat, n <= m -> n <= S m. *)
+Inductive sts:Type := 
+| STS: 
+  forall 
+  (state : Type) 
+  (trans : state -> state -> Prop), 
+  ((*init  :*) state -> Prop) -> 
+  ((*label :*) nat -> state -> Prop) ->
+  ((*serial:*) forall w : state, exists v : state, trans w v) -> sts.
+
+Definition state (M:sts):Type := 
+match M with 
+| STS state _ _ _ _ => state 
+end.
+Definition trans (M:sts): (state M) -> (state M) -> Prop := 
+match M with 
+| STS _ trans _ _ _ => trans 
+end.
+Definition init (M:sts): (state M) ->  Prop := 
+match M with 
+| STS _ _ init _ _ => init 
+end.
+Definition label (M:sts): nat -> (state M) ->  Prop := 
+match M with 
+| STS _ _ _ label _ => label 
+end.
+Definition serial (M:sts): forall w : state M, exists v : state M, trans M w v := 
+match M with 
+| STS _ _ _ _ serial => serial 
+end.
+
+Section Characerization.
+Context {H:sts}.
+
+Definition cAX := 
+  (fun (p : (state H) -> Prop) => fun (w : (state H)) =>
+      forall v : (state H), (trans H) w v -> p v): ((state H) -> Prop) -> (state H) -> Prop.
+
+Definition path := 
+(fun  (pi : nat -> (state H)) =>
+forall n : nat, (trans H) (pi n) (pi (S n))): (nat -> (state H)) -> Prop.
+
+Definition p_until := 
+  (fun (p: (state H) -> Prop)(q : (state H) -> Prop) (pi : nat -> (state H)) => 
+                    exists2 n : nat, forall m : nat, m < n -> p (pi m) & q (pi n))
+                    :((state H) -> Prop) -> ((state H) -> Prop) -> (nat -> (state H)) -> Prop.
+
+Definition pAU:= 
+  (fun (p: (state H) -> Prop) (q: (state H) -> Prop) => 
+      fun (w : (state H)) => 
+          forall (pi : nat -> (state H)), path pi -> (pi 0 = w) -> p_until p q pi) 
+      : ((state H) -> Prop) -> ((state H) -> Prop) -> (state H) -> Prop .
+
+Definition p_release:= 
+  (fun (p: (state H) -> Prop) (q: (state H) -> Prop) (pi : nat -> (state H)) =>
+  forall n : nat, (exists2 m : nat, m < n & p (pi m)) \/ q (pi n))
+  :((state H) -> Prop) -> ((state H) -> Prop) -> (nat -> (state H)) -> Prop .
+
+Definition pAR: ((state H) -> Prop) -> ((state H) -> Prop) -> (state H) -> Prop := 
+fun (p: (state H) -> Prop) (q: (state H) -> Prop) => 
+  fun (w : (state H)) =>
+    forall (pi : nat -> (state H)), path pi -> (pi 0 = w) -> p_release p q pi.
+End Characerization.
+
+Inductive form : Type :=
+| fF    : form
+| fV    : nat -> form
+| fImp  : form -> form -> form
+| fAX   : form -> form
+| fAR   : form -> form -> form 
+| fAU   : form -> form -> form.
+
+Fixpoint satisfies (M : sts) (s : form){struct s}: state M -> Prop := 
+  (match s with
+  | fF        => fun w : state M => False
+  | fV v      => fun w : state M => label M v w
+  | fImp s0 t => fun w : state M => satisfies M s0 w -> satisfies M t w
+  | fAX  s0   => fun w : state M => cAX (satisfies M s0) w
+  | fAR  s0 t => fun w : state M => pAR (satisfies M s0) (satisfies M t) w
+  | fAU  s0 t => fun w : state M => pAU (satisfies M s0) (satisfies M t) w
+  end: state M -> Prop ).
+
+
+Inductive   bool : Set :=  true : bool | false : bool.
+Definition  trans_bool (s1:bool)(s2:bool):Prop := ~ (s1 = s2).
+Definition  label_bool(v: nat)(s:bool):Prop := v = (match s with | false => 0 | true => 1 end).
+Definition  serial_bool: forall w:bool, exists v, trans_bool w v.
+intros. case w; [> eexists false|eexists true] ;compute;discriminate.
+Defined.
+Definition  init_bool(s: bool):Prop := s = false.
+Definition  model_bool: sts := 
+@STS bool trans_bool init_bool label_bool serial_bool .
+
+
+Theorem check1: forall st: state model_bool, 
+(init model_bool) st -> 
+satisfies(model_bool) (fAX (( (fV 1)))) st.
+Proof.
+  compute.
+  intros. destruct v. auto. apply H0 in H. refine (match H with end).
+Defined.
